Rewrite weakest preconditions using clkfree

src/panWeakestPreconditionScript.sml
@@ -3,177 +3,363 @@
  ***********************************************************************)
 
 Theory panWeakestPrecondition
-Ancestors panSem panPredicate
+Ancestors panSem panProps panPredicate
 
 fun elim_cases xs = EVERY (map (fn x => Cases_on x >> gvs[]) xs);
 
+Theorem state_clock_idem:
+  ∀s. s with clock := s.clock = s
+Proof
+  rw[state_component_equality]
+QED
+
 Definition hoare_def:
-  hoare P prog Q ⇔ ∀s. ∃k. P s ⇒ let (r,t) = evaluate (prog,s with clock := k)
+  hoare P prog Q ⇔ clkfree_p P ∧
+                   clkfree_q Q ∧
+                   ∀s. P s ⇒ ∃k. let (r,t) = evaluate (prog,s with clock := k)
                                  in r ≠ SOME Error ∧
                                     r ≠ SOME TimeOut ∧
-                                    ∀k'. Q (r,t with clock := k')
+                                    Q (r,t)
 End
 
 Definition wp_def:
-  wp prog Q s ⇔ ∃k. let (r,t) = evaluate (prog,s with clock := k)
+  wp prog Q s ⇔ clkfree_q Q ∧
+                ∃k. let (r,t) = evaluate (prog,s with clock := k)
                     in r ≠ SOME Error ∧
                        r ≠ SOME TimeOut ∧
-                       ∀k'. Q (r,t with clock := k')
+                       Q (r,t)
 End
 
-Theorem wp_is_weakest_precondition:
-  ∀prog Q. hoare (wp prog Q) prog Q ∧
-           ∀P. hoare P prog Q ⇔ (∀s. P s ⇒ wp prog Q s)
+Theorem wp_clkfree:
+  ∀prog Q. clkfree_p (wp prog Q)
 Proof
-  metis_tac[wp_def,hoare_def]
+  rw[clkfree_p_def,wp_def]
+QED
+
+Theorem wp_is_weakest_precondition:
+  ∀P prog Q. clkfree_p P ∧ clkfree_q Q ⇒ hoare (wp prog Q) prog Q ∧
+                                         (hoare P prog Q ⇔ (∀s. P s ⇒ wp prog Q s))
+Proof
+  metis_tac[hoare_def,wp_def,wp_clkfree]
 QED
 
 Theorem wp_monotonic:
-  ∀A B prog. (∀s. A s ⇒ B s) ⇒ (∀s. wp prog A s ⇒ wp prog B s)
+  ∀A B prog. (clkfree_q A ∧ clkfree_q B) ⇒ (∀s. A s ⇒ B s) ⇒ (∀s. wp prog A s ⇒ wp prog B s)
 Proof
-  rw[wp_def]
+  rw[wp_def,hoare_def]
   >> pairarg_tac
   >> qexists ‘k’
   >> gvs[]
 QED
 
-(* TODO FROM HERE; REVISIT DEFINITIONS ABOVE *)
+Theorem wp_conj:
+  ∀A B p. clkfree_q A ∧ clkfree_q B ⇒ (∀s. wp p (λ(r,t). A (r,t) ∧ B (r,t)) s ⇔ wp p A s ∧ wp p B s)
+Proof
+  rw[wp_def]
+  >> iff_tac
+  >> rw[]
+  >- (qexists ‘k’ >> pairarg_tac >> gvs[])
+  >- (qexists ‘k’ >> pairarg_tac >> gvs[])
+  >- metis_tac[clkfree_q_conj]
+  >> Cases_on ‘k > k'’
+  >> rpt (pairarg_tac >> gvs[])
+  >> gvs[clkfree_q_def]
+  >- (qexists ‘k’
+      >> qspecl_then [‘p’, ‘s with clock := k'’, ‘r’, ‘t’, ‘k - k'’]
+                     assume_tac evaluate_add_clock_eq
+      >> first_x_assum $ (qspecl_then [‘r’, ‘t’, ‘t.clock’, ‘k + t.clock - k'’] assume_tac)
+      >> gvs[state_clock_idem])
+  >> qexists ‘k'’
+  >> qspecl_then [‘p’, ‘s with clock := k’, ‘r'’, ‘t'’, ‘k' - k’]
+                 assume_tac evaluate_add_clock_eq
+  >> last_x_assum $ (qspecl_then [‘r’, ‘t'’, ‘t'.clock’, ‘k' + t'.clock - k’] assume_tac)
+  >> gvs[state_clock_idem]
+QED
+
+Theorem wp_disj:
+  ∀A B p. clkfree_q A ∧ clkfree_q B ⇒ (∀s. wp p (λ(r,t). A (r,t) ∨ B (r,t)) s ⇔ wp p A s ∨ wp p B s)
+Proof
+  rw[wp_def]
+  >> iff_tac
+  >> rw[]
+  >- (pairarg_tac >> gvs[]
+      >- (disj1_tac >> qexists ‘k’ >> gvs[])
+      >- (disj2_tac >> qexists ‘k’ >> gvs[]))
+  >- metis_tac[clkfree_q_disj]
+  >- (qexists ‘k’ >> pairarg_tac >> gvs[])
+  >- metis_tac[clkfree_q_disj]
+  >> qexists ‘k’
+  >> pairarg_tac
+  >> gvs[]
+QED
+
+Theorem wp_neg:
+  ∀A p. clkfree_q A ⇒ (∀s. wp p (λ(r,t). ¬A (r,t)) s ⇒ ¬wp p A s)
+Proof
+  rw[wp_def]
+  >> rw[]
+  >> rpt (pairarg_tac >> gvs[])
+  >> Cases_on ‘k > k'’
+  >- (qspecl_then [‘p’, ‘s with clock := k'’, ‘r’, ‘t’, ‘k - k'’]
+                   assume_tac evaluate_add_clock_eq
+      >> elim_cases [‘r = SOME TimeOut’]
+      >> gvs[clkfree_q_def]
+      >> first_x_assum $ (qspecl_then [‘r’, ‘t’, ‘t.clock’, ‘k + t.clock - k'’] assume_tac)
+      >> gvs[state_clock_idem])
+  >- (qspecl_then [‘p’, ‘s with clock := k’, ‘r'’, ‘t'’, ‘k' - k’]
+                   assume_tac evaluate_add_clock_eq
+      >> gvs[clkfree_q_def]
+      >> first_x_assum $ (qspecl_then [‘r’, ‘t'’, ‘t'.clock’, ‘k' + t'.clock - k’] assume_tac)
+      >> gvs[state_clock_idem])
+QED
 
 Theorem wp_skip:
-  wp Skip Q = λs. Q (NONE, s)
+  clkfree_q Q ⇒ (wp Skip Q s ⇔ Q (NONE, s))
 Proof
-  rw[FUN_EQ_THM]
-  >> iff_tac
-  >> rw[wp_def,evaluate_def]
-QED
-
-Theorem wp_seq:
-  wp (Seq p1 p2) Q res = if res = NONE then wp p1 (wp p2 Q res) res
-                                       else wp p1 (wp p2 Q res) NONE ∪ wp p1 Q res
-Proof
-  Cases_on ‘res = NONE’
-  >> rw[EXTENSION]
+  rw[wp_def,evaluate_def,clkfree_q_def]
+  >> assume_tac state_clock_idem
   >> iff_tac
   >> rw[]
-  >- (‘∃t. evaluate (p1, x) = (NONE, t) ∧ t ∈ wp p2 Q NONE’ suffices_by (metis_tac[wp_iff_postcondition])
-      >> ‘∃t. evaluate (Seq p1 p2, x) = (NONE, t) ∧ t ∈ Q’ by (metis_tac[wp_iff_postcondition])
-      >> gvs[evaluate_def]
-      >> pairarg_tac
-      >> Cases_on ‘res’
-      >> gvs[]
-      >> ‘∃t. evaluate (p2, s1) = (NONE, t) ∧ t ∈ Q’ suffices_by (metis_tac[wp_iff_postcondition])
-      >> qexists_tac ‘t’
-      >> gvs[])
-  >- (‘∃t. evaluate (Seq p1 p2, x) = (NONE, t) ∧ t ∈ Q’ suffices_by (metis_tac[wp_iff_postcondition])
-      >> ‘∃t. evaluate (p1, x) = (NONE, t) ∧ t ∈ wp p2 Q NONE’ by (metis_tac[wp_iff_postcondition])
-      >> ‘∃t'. evaluate (p2, t) = (NONE, t') ∧ t' ∈ Q’ by (metis_tac[wp_iff_postcondition])
-      >> rw[evaluate_def])
-  >- (‘(∃t. evaluate (p1, x) = (NONE, t) ∧ t ∈ wp p2 Q res) ∨ (∃t'. evaluate (p1, x) = (res, t') ∧ t' ∈ Q)’ suffices_by (metis_tac[wp_iff_postcondition])
-      >> ‘∃t. evaluate (Seq p1 p2, x) = (res, t) ∧ t ∈ Q’ by (metis_tac[wp_iff_postcondition])
-      >> gvs[evaluate_def]
-      >> pairarg_tac
-      >> Cases_on ‘res'’
-      >> gvs[]
-      >> ‘∃t. evaluate (p2, s1) = (res, t) ∧ t ∈ Q’ suffices_by (metis_tac[wp_iff_postcondition])
-      >> qexists_tac ‘t’
-      >> gvs[])
-  >- (‘∃t. evaluate (Seq p1 p2, x) = (res, t) ∧ t ∈ Q’ suffices_by (metis_tac[wp_iff_postcondition])
-      >> ‘∃t. evaluate (p1, x) = (NONE, t) ∧ t ∈ wp p2 Q res’ by (metis_tac[wp_iff_postcondition])
-      >> ‘∃t'. evaluate (p2, t) = (res, t') ∧ t' ∈ Q’ by (metis_tac[wp_iff_postcondition])
-      >> rw[evaluate_def])
-  >- (‘∃t. evaluate (Seq p1 p2, x) = (res, t) ∧ t ∈ Q’ suffices_by (metis_tac[wp_iff_postcondition])
-      >> ‘∃t. evaluate (p1, x) = (res, t) ∧ t ∈ Q’ by (metis_tac[wp_iff_postcondition])
-      >> qexists_tac ‘t’
-      >> rw[evaluate_def])
-QED
-
-Theorem wp_if:
-  wp (If e c1 c2) Q res = case res of
-                          | SOME Error => (COMPL (will_evaluate e) ∩ Q) ∪ (pred_eval e ∩ wp c1 Q (SOME Error)) ∪ (pred_compl e ∩ wp c2 Q (SOME Error))
-                          | res'       => (pred_eval e ∩ wp c1 Q res') ∪ (pred_compl e ∩ wp c2 Q res')
-Proof
-  Cases_on ‘res ≠ SOME Error’
-  >- (‘wp (If e c1 c2) Q res = (pred_eval e ∩ wp c1 Q res) ∪ (pred_compl e ∩ wp c2 Q res)’ suffices_by (elim_cases [‘res’, ‘x’])
-      >> rw[EXTENSION]
-      >> iff_tac
-      >> rw[]
-      >- (‘x ∈ will_evaluate e’ by (metis_tac[wp_if_will_evaluate])
-          >> ‘x ∈ pred_eval e ∨ x ∈ pred_compl e’ by (metis_tac[pred_eval_lem])
-          >> gvs[Once wp_def,hoare_def,evaluate_def]
-          >> first_x_assum $ (drule_then assume_tac)
-          >- (‘x ∈ pred_eval e ∧ x ∈ wp c1 Q res’ suffices_by (rw[])
-              >> ‘∃w. eval x e = SOME (ValWord w) ∧ w ≠ 0w’ by (metis_tac[pred_eval_elem])
-              >> gvs[]
-              >> ‘hoare {x} c1 Q res’ by (gvs[hoare_def])
-              >> metis_tac[all_prestates_in_wp])
-          >- (‘x ∈ pred_compl e ∧ x ∈ wp c2 Q res’ suffices_by (rw[])
-              >> ‘∃w. eval x e = SOME (ValWord w) ∧ w = 0w’ by (metis_tac[pred_compl_elem])
-              >> gvs[]
-              >> ‘hoare {x} c2 Q res’ by (gvs[hoare_def])
-              >> metis_tac[all_prestates_in_wp]))
-      >> ‘hoare {x} (If e c1 c2) Q res’ suffices_by (metis_tac[all_prestates_in_wp])
-      >> rw[hoare_def,evaluate_def]
-      >- (‘∃w. eval x e = SOME (ValWord w) ∧ w ≠ 0w’ by (metis_tac[pred_eval_elem])
-          >> ‘∃t. evaluate (c1, x) = (res, t) ∧ t ∈ Q’ by (metis_tac[wp_iff_postcondition])
-          >> gvs[])
-      >- (‘∃w. eval x e = SOME (ValWord w) ∧ w = 0w’ by (metis_tac[pred_compl_elem])
-          >> ‘∃t. evaluate (c2, x) = (res, t) ∧ t ∈ Q’ by (metis_tac[wp_iff_postcondition])
-          >> gvs[]))
+  >- (first_x_assum $ (qspecl_then [‘NONE’, ‘s’, ‘k’, ‘s.clock’] assume_tac) >> gvs[])
+  >> qexists ‘s.clock’
   >> gvs[]
-  >> rw[EXTENSION]
+QED
+
+Theorem wp_dec:
+  clkfree_q Q ⇒ (wp (Dec v sh src prog) Q s ⇔ evaluates src s ∧
+                                              subst Local v src (wp prog (reset_subst v s Q)) s)
+Proof
+  rw[wp_def,evaluate_def,clkfree_q_def,evaluates_def,subst_def,reset_subst_def]
   >> iff_tac
   >> rw[]
-  >- (‘x ∉ will_evaluate e ∨ x ∈ pred_eval e ∨ x ∈ pred_compl e’ by (metis_tac[pred_eval_lem])
-      >- (‘x ∉ will_evaluate e ∧ x ∈ Q’ suffices_by (rw[])
-          >> gvs[wp_def,hoare_def,evaluate_def]
-          >> first_x_assum $ (drule_then assume_tac)
-          >> gvs[will_evaluate_def]
-          >> elim_cases [‘eval x e’, ‘x'’, ‘w’])
-      >> gvs[Once wp_def,hoare_def,evaluate_def]
-      >> first_x_assum $ (drule_then assume_tac)
-      >- (‘x ∈ pred_eval e ∧ x ∈ wp c1 Q (SOME Error)’ suffices_by (rw[])
-          >> ‘∃w. eval x e = SOME (ValWord w) ∧ w ≠ 0w’ by (metis_tac[pred_eval_elem])
-          >> gvs[]
-          >> ‘hoare {x} c1 Q (SOME Error)’ by (gvs[hoare_def])
-          >> metis_tac[all_prestates_in_wp])
-      >- (‘x ∈ pred_compl e ∧ x ∈ wp c2 Q (SOME Error)’ suffices_by (rw[])
-          >> ‘∃w. eval x e = SOME (ValWord w) ∧ w = 0w’ by (metis_tac[pred_compl_elem])
-          >> gvs[]
-          >> ‘hoare {x} c2 Q (SOME Error)’ by (gvs[hoare_def])
-          >> metis_tac[all_prestates_in_wp]))
-  >> ‘hoare {x} (If e c1 c2) Q (SOME Error)’ suffices_by (metis_tac[all_prestates_in_wp])
-  >> rw[hoare_def,evaluate_def]
-  >- (gvs[will_evaluate_def]
-      >> elim_cases [‘eval x e’, ‘x'’, ‘w’])
-  >- (‘∃w. eval x e = SOME (ValWord w) ∧ w ≠ 0w’ by (metis_tac[pred_eval_elem])
-      >> ‘∃t. evaluate (c1, x) = (SOME Error, t) ∧ t ∈ Q’ by (metis_tac[wp_iff_postcondition])
+  >> assume_tac state_clock_idem
+  >> assume_tac eval_upd_clock_eq
+  >> elim_cases [‘eval s src’]
+  >> rpt (pairarg_tac >> gvs[])
+  >> rw[]
+  >- (first_x_assum $ (qspecl_then [‘r'’,
+                                    ‘s' with locals := res_var s'.locals (v,FLOOKUP s.locals v)’,
+                                    ‘k1’, ‘k2’] assume_tac)
       >> gvs[])
-  >- (‘∃w. eval x e = SOME (ValWord w) ∧ w = 0w’ by (metis_tac[pred_compl_elem])
-      >> ‘∃t. evaluate (c2, x) = (SOME Error, t) ∧ t ∈ Q’ by (metis_tac[wp_iff_postcondition])
-      >> gvs[])
+  >> qexists ‘k’
+  >> gvs[]
 QED
 
 Theorem wp_assign:
-  wp (Assign v src) Q res = case res of
-                            | NONE       => valid_value v src ∩ subst v src Q
-                            | SOME Error => Q DIFF valid_value v src
-                            | _          => ∅
+  clkfree_q Q ⇒ (wp (Assign k v src) Q s ⇔ valid_value k v src s ∧
+                                           subst k v src (λs. Q (NONE, s)) s)
 Proof
-  Cases_on ‘res’
-  >- (rw[EXTENSION]
-      >> iff_tac
-      >> rw[]
-      >- metis_tac[wp_assign_valid_value]
-      >- metis_tac[wp_assign_subst]
-      >> ‘hoare {x} (Assign v src) Q NONE’ suffices_by (metis_tac[all_prestates_in_wp])
-      >> gvs[valid_value_def,subst_def,hoare_def,evaluate_def]
-      >> pairarg_tac
-      >> elim_cases [‘eval x src’])
-  >> Cases_on ‘x’
-  >- gvs[EXTENSION,wp_error_invalid]
-  >> gvs[EXTENSION,wp_iff_postcondition,evaluate_def]
+  Cases_on ‘k’
+  >> rw[wp_def,evaluate_def,clkfree_q_def,valid_value_def,subst_def]
+  >> iff_tac
   >> rw[]
-  >> elim_cases [‘eval x src’, ‘is_valid_value x.locals v x'’]
+  >> assume_tac state_clock_idem
+  >> assume_tac eval_upd_clock_eq
+  >> elim_cases [‘eval s src’]
+  >- elim_cases [‘is_valid_value s.locals v x’]
+  >- (elim_cases [‘is_valid_value s.locals v x’]
+      >> first_x_assum $ (qspecl_then [‘NONE’, ‘s with locals := s.locals |+ (v,x)’,
+                                       ‘k’, ‘s.clock’] assume_tac)
+      >> gvs[])
+  >- (qexists ‘s.clock’ >> gvs[])
+  >- elim_cases [‘is_valid_value s.globals v x’]
+  >- (elim_cases [‘is_valid_value s.globals v x’]
+      >> first_x_assum $ (qspecl_then [‘NONE’, ‘s with globals := s.globals |+ (v,x)’,
+                                       ‘k’, ‘s.clock’] assume_tac)
+      >> gvs[])
+  >> qexists ‘s.clock’
+  >> gvs[]
 QED
 
-val _ = export_theory();
+Theorem wp_store:
+  clkfree_q Q ⇒ (wp (Store dest src) Q s ⇔ ∃addr val. evaluates_to dest (ValWord addr) s ∧
+                                                      evaluates_to src val s ∧
+                                                      addr_in_mem addr val s ∧
+                                                      mem_subst addr val (λs. Q (NONE, s)) s)
+Proof
+  rw[wp_def,evaluate_def,clkfree_q_def,evaluates_to_def,addr_in_mem_def,mem_subst_def]
+  >> iff_tac
+  >> rw[]
+  >> assume_tac state_clock_idem
+  >> assume_tac eval_upd_clock_eq
+  >> elim_cases [‘eval s src’, ‘eval s dest’]
+  >- elim_cases [‘x’]
+  >- (elim_cases [‘x'’, ‘w’, ‘mem_stores c (flatten x) s.memaddrs s.memory’]
+      >> first_x_assum $ (qspecl_then [‘NONE’, ‘s with memory := x'’,
+                                       ‘k’, ‘s.clock’] assume_tac)
+      >> gvs[])
+  >> qexists ‘s.clock’
+  >> gvs[]
+QED
+
+Theorem wp_store32:
+  clkfree_q Q ⇒ (wp (Store32 dest src) Q s ⇔ ∃addr val. evaluates_to dest (ValWord addr) s ∧
+                                                        evaluates_to src (ValWord val) s ∧
+                                                        addr_in_mem_32 addr val s ∧
+                                                        mem_subst_32 addr val (λs. Q (NONE, s)) s)
+Proof
+  rw[wp_def,evaluate_def,clkfree_q_def,evaluates_to_def,addr_in_mem_32_def,mem_subst_32_def]
+  >> iff_tac
+  >> rw[]
+  >> assume_tac state_clock_idem
+  >> assume_tac eval_upd_clock_eq
+  >> elim_cases [‘eval s src’, ‘eval s dest’]
+  >- elim_cases [‘x’]
+  >- (elim_cases [‘x’, ‘x'’, ‘w’, ‘w'’, ‘mem_store_32 s.memory s.memaddrs s.be c' (w2w c)’]
+      >> first_x_assum $ (qspecl_then [‘NONE’, ‘s with memory := x’,
+                                       ‘k’, ‘s.clock’] assume_tac)
+      >> gvs[])
+  >> qexists ‘s.clock’
+  >> gvs[]
+QED
+
+Theorem wp_storebyte:
+  clkfree_q Q ⇒ (wp (StoreByte dest src) Q s ⇔ ∃addr val. evaluates_to dest (ValWord addr) s ∧
+                                                          evaluates_to src (ValWord val) s ∧
+                                                          addr_in_mem_byte addr val s ∧
+                                                          mem_subst_byte addr val (λs. Q (NONE, s)) s)
+Proof
+  rw[wp_def,evaluate_def,clkfree_q_def,evaluates_to_def,addr_in_mem_byte_def,mem_subst_byte_def]
+  >> iff_tac
+  >> rw[]
+  >> assume_tac state_clock_idem
+  >> assume_tac eval_upd_clock_eq
+  >> elim_cases [‘eval s src’, ‘eval s dest’]
+  >- elim_cases [‘x’]
+  >- (elim_cases [‘x’, ‘x'’, ‘w’, ‘w'’, ‘mem_store_byte s.memory s.memaddrs s.be c' (w2w c)’]
+      >> first_x_assum $ (qspecl_then [‘NONE’, ‘s with memory := x’,
+                                       ‘k’, ‘s.clock’] assume_tac)
+      >> gvs[])
+  >> qexists ‘s.clock’
+  >> gvs[]
+QED
+
+Theorem wp_seq:
+  clkfree_q Q ⇒ (wp (Seq p1 p2) Q s ⇔ wp p1 (λ(r,t). r = NONE ∧ (wp p2 Q) t) s ∨
+                                      wp p1 (λ(r,t). r ≠ NONE ∧ Q (r,t)) s)
+Proof
+  rw[wp_def,evaluate_def,clkfree_q_def]
+  >> iff_tac
+  >> rw[]
+  >> rpt (pairarg_tac >> gvs[])
+  >- (Cases_on ‘res’
+      >> gvs[]
+      >- (disj1_tac
+          >> qspecl_then [‘s with clock := k’, ‘s1’, ‘NONE’, ‘p1’]
+                         assume_tac (GEN_ALL evaluate_min_clock)
+          >> gvs[]
+          >> qexists ‘k' + s1.clock’
+          >> rpt (pairarg_tac >> gvs[])
+          >> qspecl_then [‘p1’, ‘s with clock := k'’, ‘NONE’, ‘s1 with clock := 0’, ‘s1.clock’]
+                         assume_tac evaluate_add_clock_eq
+          >> gvs[]
+          >> qexists ‘s1.clock’
+          >> gvs[state_clock_idem])
+      >> disj2_tac
+      >> rw[]
+      >- (first_x_assum $ (qspecl_then [‘r’, ‘s'’, ‘k1’, ‘k2’] assume_tac) >> gvs[])
+      >> qexists ‘k’
+      >> gvs[])
+  >- (qspecl_then [‘s with clock := k’, ‘t’, ‘NONE’, ‘p1’]
+                  assume_tac (GEN_ALL evaluate_min_clock)
+      >> gvs[]
+      >> qexists ‘k'' + k'’
+      >> qspecl_then [‘p1’, ‘s with clock := k''’, ‘NONE’, ‘t with clock := 0’, ‘k'’]
+                     assume_tac evaluate_add_clock_eq
+      >> gvs[])
+  >> qexists ‘k’
+  >> gvs[]
+QED
+
+Theorem wp_if:
+  clkfree_q Q ⇒ (wp (If e c1 c2) Q s ⇔ (evaluates_to_word  e s)             ∧
+                                       (evaluates_to_true  e s ⇒ wp c1 Q s) ∧
+                                       (evaluates_to_false e s ⇒ wp c2 Q s))
+Proof
+  rw[wp_def,evaluate_def,evaluates_to_word_def,evaluates_to_true_def,evaluates_to_false_def]
+  >> iff_tac
+  >> rw[]
+  >> assume_tac eval_upd_clock_eq
+  >- elim_cases [‘eval s e’, ‘x’, ‘w’]
+  >- (qexists ‘k’ >> gvs[])
+  >> elim_cases [‘w = 0w’]
+  >> qexists ‘k’
+  >> gvs[]
+QED
+
+Theorem wp_break:
+  clkfree_q Q ⇒ (wp Break Q s ⇔ Q (SOME Break,s))
+Proof
+  rw[wp_def,evaluate_def,clkfree_q_def]
+  >> assume_tac state_clock_idem
+  >> iff_tac
+  >> rw[]
+  >- (first_x_assum $ (qspecl_then [‘SOME Break’, ‘s’, ‘k’, ‘s.clock’] assume_tac) >> gvs[])
+  >> qexists ‘s.clock’
+  >> gvs[]
+QED
+
+Theorem wp_continue:
+  clkfree_q Q ⇒ (wp Continue Q s ⇔ Q (SOME Continue,s))
+Proof
+  rw[wp_def,evaluate_def,clkfree_q_def]
+  >> assume_tac state_clock_idem
+  >> iff_tac
+  >> rw[]
+  >- (first_x_assum $ (qspecl_then [‘SOME Continue’, ‘s’, ‘k’, ‘s.clock’] assume_tac) >> gvs[])
+  >> qexists ‘s.clock’
+  >> gvs[]
+QED
+
+Theorem wp_raise:
+  clkfree_q Q ⇒ (wp (Raise eid e) Q s ⇔ ∃sh val. has_eshape eid sh s ∧
+                                                 evaluates_to e val s ∧
+                                                 shape_of val = sh ∧
+                                                 size_of_shape sh ≤ 32 ∧
+                                                 Q (SOME (Exception eid val),empty_locals s))
+Proof
+  rw[wp_def,evaluate_def,clkfree_q_def,has_eshape_def,evaluates_to_def]
+  >> iff_tac
+  >> rw[]
+  >> rpt (pairarg_tac >> gvs[])
+  >> assume_tac state_clock_idem
+  >> assume_tac eval_upd_clock_eq
+  >- (elim_cases [‘FLOOKUP s.eshapes eid’, ‘eval s e’, ‘shape_of x' = x’,
+                  ‘size_of_shape (shape_of x') ≤ 32’]
+      >> first_x_assum $ (qspecl_then [‘SOME (Exception eid x')’, ‘s with locals := FEMPTY’,
+                                       ‘s.clock’, ‘k’] assume_tac)
+      >> gvs[empty_locals_def])
+  >> qexists ‘s.clock’
+  >> gvs[]
+QED
+
+Theorem wp_return:
+  clkfree_q Q ⇒ (wp (Return e) Q s ⇔ ∃val. evaluates_to e val s ∧
+                                           size_of_shape (shape_of val) ≤ 32 ∧
+                                           Q (SOME (Return val),empty_locals s))
+Proof
+  rw[wp_def,evaluate_def,clkfree_q_def,evaluates_to_def]
+  >> iff_tac
+  >> rw[]
+  >> rpt (pairarg_tac >> gvs[])
+  >> assume_tac state_clock_idem
+  >> assume_tac eval_upd_clock_eq
+  >- (elim_cases [‘eval s e’, ‘size_of_shape (shape_of x) ≤ 32’]
+      >> first_x_assum $ (qspecl_then [‘SOME (Return x)’, ‘s with locals := FEMPTY’,
+                                       ‘s.clock’, ‘k’] assume_tac)
+      >> gvs[empty_locals_def])
+  >> qexists ‘s.clock’
+  >> gvs[]
+QED
+
+Theorem wp_annot:
+  clkfree_q Q ⇒ (wp (Annot a b) Q s ⇔ Q (NONE,s))
+Proof
+  rw[wp_def,evaluate_def,clkfree_q_def]
+  >> assume_tac state_clock_idem
+  >> iff_tac
+  >> rw[]
+  >- (first_x_assum $ (qspecl_then [‘NONE’, ‘s’, ‘k’, ‘s.clock’] assume_tac) >> gvs[])
+  >> qexists ‘s.clock’
+  >> gvs[]
+QED
